Added valid. Removed options.

Common/Rc.v
@@ -1,3 +1,4 @@
+Require Import Events.
 Require Import Smallstep.
 Require Import Behavior.
 Require Import Coq.Lists.List.
@@ -13,7 +14,6 @@ Require Import Coq.Program.Basics.
    in Main.robust_compilation_static_compromise.
  *)
 
-
 (* 
    Some Global definitions.
  *)
@@ -28,38 +28,11 @@ Axiom turn : program_behavior -> interface -> Prop.
 Axiom icomplete : interface -> Prop.
 (* check if the union of two interfaces is complete *)
 Definition icomplete2 (i1 i2:interface) := icomplete (i1++i2).
+Definition contained {A} (i1 i2: list A) := exists i3, i1++i3=i2.
 (* TODO check this *)
 Axiom unique_interfaces :
   forall (i1 i2 i3:interface),
     icomplete2 i1 i3 -> icomplete2 i2 i3 -> i1=i2.
-
-(* 
-   option monad stuff
- *)
-Definition map {A B} (f: A -> B) (o: option A) : option B :=
-  match o with
-  | Some a => Some (f a)
-  | None => None
-  end.
-
-Definition map_compose :
-  forall {A B C} (f1: A -> B) (f2: B -> C) (x:option A),
-    map f2 (map f1 x) = map (compose f2 f1) x.
-Proof.
-  destruct x; auto.
-Qed.
-
-Definition propagate {A B} (f: A -> option B) (op:option A) : option B :=
-  match op with
-  | Some p => f p
-  | None => None
-  end.
-
-Definition behaves (o: option semantics) b : Prop :=
-  match o with
-  | Some p => program_behaves p b
-  | None => False
-  end.
 
 
 (* 
@@ -69,65 +42,92 @@ Definition behaves (o: option semantics) b : Prop :=
 (* Signature of basic things expected in a language *)
 Module Type Lang.
   (* Type of programs, complete or partial *)
-  Axiom program : Type.
-  Axiom get_interface: program -> interface. (* CH: TODO replace with has_interface relation between well-formed programs
-                                                         and their corresponding interfaces; has_interface is a
-                                                         (not necessarily computable) partial function *)
+  Parameter program : Type.
+  (* relation between well-formed programs and their corresponding
+     interfaces; has_interface is a (not necessarily computable) 
+     partial function *)
+  Parameter valid : program -> Prop.
+  Parameter get_interface: program -> interface.
+  (* Parameter get_interface_spec: *)
+  (*   forall p, valid p -> exists i, get_interface p = Some i. *)
+  
   (* checks if a program has a complete interface *)
-  Axiom complete: program -> Prop.
+  Parameter complete: program -> Prop.
+  (* Parameter complete_spec: *)
+  (*   forall p, valid p -> exists i, get_interface p = Some i /\ complete p = icomplete i. *)
+  
   (* checks if two programs linked together form a complete program *)
-  Axiom complete2: program -> program -> Prop.
+  Parameter complete2: program -> program -> Prop.
 
+  (* Parameter state: Type. *)
+  (* Parameter genvtype: Type. *)
+  (* Parameter step : genvtype -> state -> trace -> state -> Prop. *)
+  (* Parameter initial_state : program -> state -> Prop. *)
+  (* Parameter final_state: state -> Prop. *)
+  (* Parameter globalenv: program -> genvtype. *)
+
+  (* Definition sem (p: program) : semantics := *)
+  (*   let ge := globalenv p in *)
+  (*   Semantics_gen step (initial_state p) final_state ge. *)
+  
   (* complete semantics: takes a complete program *)
-  Axiom sem: program -> option semantics.
-  (* Axiom sem_complete: *)
-  (*   forall (p:program), *)
-  (*     complete p -> exists s, sem (Some p) = Some s. *)
-
+  Parameter sem: program -> semantics.
+  (* any program has a semantics, if the program is ill-formed it still has a behavior.
+     e.g. a program without any initial state satisfies program_goes_initially_wrong *)
+  
   (* partial semantics: takes a program and a matching interface.
      The interface of the program together with the matching interface
      is complete. *)
-  Axiom psem: interface -> program -> option semantics.
-  (* Axiom psem_complete: *)
-  (*   forall psi (p:program), *)
-  (*     icomplete2 psi (get_interface p) -> exists s, psem (Some p) psi = Some s. *)
-  Definition osem (op: option program) := propagate sem op.
-  Definition opsem i (op: option program) := propagate (psem i) op.
+  Parameter psem: interface -> program -> semantics.
 
   (* Axiom idefinability: forall (i:interface), exists (p:program), get_interface p = i. *)
 End Lang.
 
 (* Every language is a subtype of Lang and implements its signature *)
-(* Note: nothing is really implemented, we just give type signatures *)
+(* Note: most things are just axioms *)
 
 (* Intermediate *)
 Module I <: Lang.
   Axiom program : Type.
+  Axiom valid: program -> Prop.
   Axiom get_interface: program -> interface.
-  Definition complete (p:program) := icomplete (get_interface p).
-  Definition complete2 (p1 p2:program) := icomplete2 (get_interface p1) (get_interface p2).
-  Axiom sem: program -> option semantics.
-  Axiom psem: interface -> program -> option semantics.
-  Definition osem (op: option program) := propagate sem op.
-  Definition opsem i (op: option program) := propagate (psem i) op.
+  Definition complete (p:program) :=
+    valid p /\ icomplete (get_interface p).
+  Definition complete2 (p1 p2:program) :=
+    valid p1 /\
+    valid p2 /\
+    icomplete2 (get_interface p1) (get_interface p2).
+    
+  Axiom sem: program -> semantics.
+  Axiom psem: interface -> program -> semantics.
 
-  (* linking of two partial programs, returns a complete program *)
-  Axiom link: program -> program -> option program.
-  Axiom link_prepost:
+  (* linking of two partial programs, this is restricted to the
+     complete case, we could generalize by asking that p1 and p2 are
+     compatible *)
+  Axiom link: program -> program -> program.
+  Axiom link_spec:
     forall (p1 p2:program),
-      complete2 p1 p2 -> exists p, (link p1 p2 = Some p) /\ (get_interface p = (get_interface p1) ++ (get_interface p2)).
+      valid p1 /\ valid p2 /\ complete2 p1 p2 ->
+      exists (p:program),
+        (get_interface p1) ++ (get_interface p2) = (get_interface p) /\
+        valid p /\ complete p.
 
+  (* only for the safe case *)
+  (* TODO has p to be FD? *)
   Axiom decomposition:
     forall beh (c p:I.program),
-      behaves (osem (I.link c p)) beh
-      ->
-      behaves (opsem (I.get_interface c) (Some p)) beh. (* CH: Some not needed *)
-
-  Definition fully_defined (psi:interface) (p:program) :=
-    forall (beh:program_behavior) (c:program),
-      get_interface c = psi ->
       complete2 c p ->
-      behaves (osem (link c p)) beh ->
+      program_behaves (sem (link c p)) beh ->
+      not_wrong beh ->
+      program_behaves (psem (get_interface c) p) beh.
+  
+  Definition fully_defined (psi:interface) (p:program) :=
+    valid p ->
+    icomplete2 psi (get_interface p) ->
+    forall (beh:program_behavior) (c:program),
+      valid c ->
+      get_interface c = psi ->
+      program_behaves (sem (link c p)) beh ->
       (turn beh (get_interface p) ->
        not_wrong beh).
 End I.
@@ -135,104 +135,123 @@ End I.
 (* Source *)
 Module S <: Lang.
   Axiom program : Type.
+  Axiom valid: program -> Prop.
   Axiom get_interface: program -> interface.
-  Definition complete (p:program) := icomplete (get_interface p).
-  Definition complete2 (p1 p2:program) := icomplete2 (get_interface p1) (get_interface p2).
-  Axiom sem: program -> option semantics.
-  Axiom psem: interface -> program -> option semantics.
-  Definition osem (op: option program) := propagate sem op.
-  Definition opsem i (op: option program) := propagate (psem i) op.
+  Definition complete (p:program) :=
+    valid p /\ icomplete (get_interface p).
+  Definition complete2 (p1 p2:program) :=
+    valid p1 /\
+    valid p2 /\
+    icomplete2 (get_interface p1) (get_interface p2).
+  Axiom sem: program -> semantics.
+  Axiom psem: interface -> program -> semantics.
 
-  Axiom link: program -> program -> option program.
+  Axiom link: program -> program -> program.
 
   Definition fully_defined (psi:interface) (p:program) :=
+    valid p /\
+    icomplete2 psi (get_interface p) /\
     forall (beh:program_behavior) (c:program),
+      valid c ->
       get_interface c = psi ->
-      complete2 c p ->
-      behaves (osem (link c p)) beh ->
+      program_behaves (sem (link c p)) beh ->
       (turn beh (get_interface p) ->
        not_wrong beh).
 
+  (* TODO can beh be UB? *)
+  (* TODO if P is FD then we can argue that beh is not wrong *)
   Axiom definability:
     forall (beh:program_behavior) (psi:interface) (p:program),
+      valid p ->
       icomplete2 psi (get_interface p) ->
-      behaves (psem psi p) beh ->
+      program_behaves (psem psi p) beh ->
+      (* not_wrong beh -> *)
       exists (c:program),
-        behaves (osem (link c p)) beh /\ get_interface c = psi.
+        program_behaves (sem (link c p)) beh /\ valid c /\ get_interface c = psi.
 End S.
 
 (* Source to Intermediate *)
 Module SI.
+  (* TODO
+     compcert defined the compiler as:
+     - a function transf_c_program (p: Csyntax.program) : res Asm.program
+     - a relation match_prog: Csyntax.program -> Asm.program -> Prop
+     and proves their equivalence in transf_c_program_match.
+ *)
   Axiom compile : S.program -> I.program.
-  Axiom compile_complete :
-    forall p1 p2,
-      S.complete p1 -> compile p1 = p2 -> I.complete p2.
-  
-  Axiom compiler_interfaces:
-    forall (p1:S.program),
-      S.get_interface p1 = I.get_interface (compile p1).
+  Axiom compile_spec:
+    forall (p:S.program),
+      S.valid p ->
+      I.valid (compile p) /\ S.get_interface p = I.get_interface (compile p).
 
-  (* exact cc preserves also UB *)
+  (* TODO does it preserve also UB? *)
   Axiom compiler_correctness :
     forall beh (p:S.program) (psi:interface),
-      behaves (I.psem psi (SI.compile p)) beh ->
-      behaves (S.psem psi p) beh.
+      S.valid p ->
+      icomplete2 psi (S.get_interface p) ->
+      program_behaves (I.psem psi (SI.compile p)) beh ->
+      program_behaves (S.psem psi p) beh.
 
-  (* TODO This is too syntactic, it should be stated in terms of equivalent behaviors *)
+  (* TODO This is too syntactic, it should be stated in terms of 
+     equivalent behaviors *)
   (* Only needed for RC variant *)
   Axiom separate_compilation:
     forall (P Q: S.program),
-      map SI.compile (S.link Q P) = I.link (SI.compile Q) (SI.compile P).
+      S.complete2 Q P ->
+      SI.compile (S.link Q P) = I.link (SI.compile Q) (SI.compile P).
 
   (* RC between S and I *)
   Definition RC:
     forall (c:I.program) (P:S.program) (beh:program_behavior),
-      icomplete2 (I.get_interface c) (S.get_interface P) ->
       S.fully_defined (I.get_interface c) P ->
-      behaves (I.osem (I.link c (SI.compile P))) beh
-      ->
+      I.valid c ->
+      program_behaves (I.sem (I.link c (SI.compile P))) beh ->
+      not_wrong beh ->
       exists C,
-        behaves (S.osem (S.link C P)) beh /\ S.complete2 C P.
+        program_behaves (S.sem (S.link C P)) beh /\ S.complete2 C P.
   Proof.
-    intros c P b Hcomplete SFD H.
+    intros c P b [HvalP [Hcomplete H1]] Hvalc H Hsafe.
+    destruct (compile_spec P HvalP) as [H2 Hcompint].
     apply I.decomposition in H.
-    destruct (I.link_prepost c (SI.compile P)) as [p [H1 H2]].
-    unfold I.complete2.
-    rewrite <- SI.compiler_interfaces.
-    auto.
     apply (SI.compiler_correctness b P (I.get_interface c)) in H.
-    apply S.definability in H.
-    destruct H as [C [Hb Hif]].
+    destruct (S.definability b (I.get_interface c) P HvalP Hcomplete H) as [C [Hb [HvalC Hif]]].
+    auto.
     exists C.
-    split.
-    auto.
+    split; auto.
+    unfold S.complete2.
     rewrite <- Hif in Hcomplete.
-    auto.
+    repeat split; auto.
+    all: auto.
+    repeat split;auto.
+    rewrite <- Hcompint.
     auto.
   Qed.
 
+  (* Require Import Coq.Logic.Classical. *)
+
   (* This is proved using RC. *)
   Definition FD_preservation:
-    forall (psi:interface) (p:S.program),
-      S.fully_defined psi p ->
-      I.fully_defined psi (SI.compile p).
+    forall (psi:interface) (P:S.program),
+      S.fully_defined psi P ->
+      I.fully_defined psi (SI.compile P).
   Proof.
-    intros psi p SFD.
-    intros b c Hpsi Hcomplete H1.
-    unfold I.complete2 in Hcomplete.
-    rewrite <- SI.compiler_interfaces in Hcomplete.
-    destruct (SI.RC c p b Hcomplete) as [C [H2 H3]].
-    rewrite Hpsi.
-    apply SFD.
-    assumption.
-    unfold S.fully_defined in SFD.
-    rewrite <- SI.compiler_interfaces.
-    apply (SFD b C).
-    unfold S.complete2 in H3.  
-    destruct (unique_interfaces (I.get_interface c) (S.get_interface C) (S.get_interface p)); auto.
-    auto.
-    auto.
-  Qed.
+    intros psi P SFD.
+    (* assert (SFD2 := SFD). *)
+    unfold I.fully_defined.
+    intros p Hcomplete b c Hvalc Hif Hbeh.
+    rewrite <- Hif in SFD.
+    destruct (SI.RC c P b SFD Hvalc) as [C [H3 H4]].
+    (* destruct (classic (turn b (S.get_interface p))). *)
+    (* destruct (classic (not_wrong b )). *)
+    (* destruct SFD as [Hvalp [H88 HFD]]. *)
+    (* destruct (compile_spec p Hvalp) as [Hvalcomp Hint2]. *)
+    (* rewrite <- Hint2. *)
+    (* destruct SFD as [Hvalp [H88 HFD]]. *)
+    (* destruct (compile_spec p Hvalp) as [Hvalcomp Hint]. *)
+    (* apply not_all_ex_not in H0 as [b1 NW]. *)
+    (* destruct (compile_spec p Hvalp) as [Hvalcomp Hint]. *)
+    (* destruct (unique_interfaces (I.get_interface c) (S.get_interface C) (S.get_interface p)). *)
+  Admitted.
 End SI.
 
 
@@ -240,25 +259,23 @@ End SI.
 (* Micro-policies target language *)
 Module MP <: Lang.
   Axiom program : Type.
+  Axiom valid: program -> Prop.
   Axiom get_interface: program -> interface.
   Definition complete (p:program) := icomplete (get_interface p).
   Definition complete2 (p1 p2:program) := icomplete2 (get_interface p1) (get_interface p2).
-  Axiom sem: program -> option semantics.
-  Axiom psem: interface -> program -> option semantics.
-  Definition osem (op: option program) := propagate sem op.
-  Definition opsem i (op: option program) := propagate (psem i) op.
+  Axiom sem: program -> semantics.
+  Axiom psem: interface -> program -> semantics.
 End MP.
 
 (* Software Fault Isolation target language *)
 Module SFI <: Lang.
   Axiom program : Type.
+  Axiom valid: program -> Prop.
   Axiom get_interface: program -> interface.
   Definition complete (p:program) := icomplete (get_interface p).
   Definition complete2 (p1 p2:program) := icomplete2 (get_interface p1) (get_interface p2).
-  Axiom sem: program -> option semantics.
-  Axiom psem: interface -> program -> option semantics.
-  Definition osem (op: option program) := propagate sem op.
-  Definition opsem i (op: option program) := propagate (psem i) op.
+  Axiom sem: program -> semantics.
+  Axiom psem: interface -> program -> semantics.
 End SFI.
 
 
@@ -267,41 +284,50 @@ End SFI.
 Module Type IT.
   Declare Module T : Lang.
   
+  (* TODO
+     compcert defined the compiler as:
+     - a function transf_c_program (p: Csyntax.program) : res Asm.program
+     - a relation match_prog: Csyntax.program -> Asm.program -> Prop
+     and proves their equivalence in transf_c_program_match.
+ *)
   (* TODO IT.compile must be a refinement compiler *)
-  Axiom compile : I.program -> T.program.
+  Parameter compile : I.program -> T.program.
+  Axiom compile_spec:
+    forall (p:I.program),
+      I.valid p -> T.valid (compile p) /\
+                   I.get_interface p = T.get_interface (compile p).
   
   (* takes a complete program and produces a partial one
    This is an important ingredient for the simulation relation.
    For MP the relation corresponds with this function actually.
    For SFI the relation contains additional elements.
    *)
-  Axiom partialize: interface -> T.program -> option T.program.
-  Axiom partialize_post:
-    forall (p:T.program) psi,
-    exists pp, 
-      (T.get_interface p) = (T.get_interface pp)++psi ->
-      partialize psi p = Some pp.
-  Definition opartialize psi (op: option T.program) := propagate (partialize psi) op.
+  Parameter partialize: interface -> T.program -> T.program.
+  Parameter partialize_spec:
+    forall psi (p:T.program),
+      T.valid p ->
+      contained psi (T.get_interface p) ->
+      (T.get_interface p) = (T.get_interface (partialize psi p))++psi.
 
   (* 
      The following properties are special because they depend on
      compiling the complete intermediate program.
    *)
-  Axiom special_decomposition :
+  Parameter special_decomposition :
     forall beh (c p:I.program),
       I.fully_defined (I.get_interface c) p ->
-      let ip := map compile (I.link c p) in
-      behaves (T.osem ip) beh
+      let ip := compile (I.link c p) in
+      program_behaves (T.sem ip) beh
       ->
-      behaves (T.opsem (I.get_interface c) (opartialize (I.get_interface c) ip)) beh.
+      program_behaves (T.psem (I.get_interface c) (partialize (I.get_interface c) ip)) beh.
 
-  Axiom special_compiler_correctness:
+  Parameter special_compiler_correctness:
     forall beh (c p:I.program),
       I.fully_defined (I.get_interface c) p ->
       let ip := I.link c p in
-      let tp := opartialize (I.get_interface c) (map compile ip) in
-      behaves (T.opsem (I.get_interface c) tp) beh ->
-      behaves (I.opsem (I.get_interface c) (Some p))  beh.
+      let tp := partialize (I.get_interface c) (compile ip) in
+      program_behaves (T.psem (I.get_interface c) tp) beh ->
+      program_behaves (I.psem (I.get_interface c) p)  beh.
 End IT.
 
 (* Micro-policies compiler *)
@@ -309,54 +335,63 @@ Module MPC <: IT.
   Module T := MP.
   
   Axiom compile : I.program -> T.program.
-  Axiom compile_complete :
-    forall p1 p2,
-      I.complete p1 -> compile p1 = p2 -> T.complete p2.
-  
-  Axiom compiler_interfaces:
-    forall (p1:I.program),
-      I.get_interface p1 = T.get_interface (compile p1).
+  Axiom compile_spec:
+    forall (p:I.program),
+      I.valid p -> T.valid (compile p) /\
+                   I.get_interface p = T.get_interface (compile p).
 
-  Axiom partialize: interface -> T.program -> option T.program.
-  Axiom partialize_post:
-    forall (p:T.program) psi,
-    exists pp,
-      (T.get_interface p) = (T.get_interface pp)++psi ->
-      partialize psi p = Some pp.
-  Definition opartialize psi (op: option T.program) := propagate (partialize psi) op.
+  Axiom partialize: interface -> T.program -> T.program.
+  Axiom partialize_spec:
+    forall psi (p:T.program),
+      T.valid p ->
+      contained psi (T.get_interface p) ->
+      (T.get_interface p) = (T.get_interface (partialize psi p))++psi.
 
+  (* Axiom forward_simulation_behavior: *)
+  (*   forall p psi, *)
+  (*     T.complete p -> *)
+  (*     contained psi (T.get_interface p) -> *)
+  (*     exists (cs ps:semantics) f, f=forward_simulation cs ps. *)
+    
+  (*   Theorem forward_simulation_behavior: *)
+  (*   forall p psi cs ps, *)
+  (*     T.sem p = Some cs -> *)
+  (*     T.opsem psi (partialize psi p) = Some ps -> *)
+  (*     forward_simulation cs ps -> *)
+  (*     forall beh1, program_behaves cs beh1 -> *)
+  (*                  program_behaves ps beh1. *)
+  (* Proof. *)
+  (*   intros p psi cs ps Hsem Hpsem Hfs b H1. *)
+    
   (* TODO prove assuming simulation *)
   Axiom partialize_decomposition:
     forall beh (p:T.program) psi,
-      behaves (T.osem (Some p)) beh
+      program_behaves (T.sem p) beh
       ->
-      behaves (T.opsem psi (opartialize psi (Some p))) beh.
+      program_behaves (T.psem psi (partialize psi p)) beh.
   
   (* we can prove special decomposition using the more general
      decomposition *)
   Definition special_decomposition :
     forall beh (c p:I.program),
       I.fully_defined (I.get_interface c) p ->
-      let ip := map compile (I.link c p) in
-      behaves (T.osem ip) beh
+      let ip := compile (I.link c p) in
+      program_behaves (T.sem ip) beh
       ->
-      behaves (T.opsem (I.get_interface c) (opartialize (I.get_interface c) ip)) beh.
+      program_behaves (T.psem (I.get_interface c) (partialize (I.get_interface c) ip)) beh.
   Proof.
     intros b c p IFD ip H.
-    destruct ip.
     apply partialize_decomposition.
     assumption.
-    simpl in H.
-    auto.
   Qed.
 
   Axiom special_compiler_correctness:
     forall beh (c p:I.program),
       I.fully_defined (I.get_interface c) p ->
       let ip := I.link c p in
-      let tp := opartialize (I.get_interface c) (map compile ip) in
-      behaves (T.opsem (I.get_interface c) tp) beh ->
-      behaves (I.opsem (I.get_interface c) (Some p))  beh.
+      let tp := partialize (I.get_interface c) (compile ip) in
+      program_behaves (T.psem (I.get_interface c) tp) beh ->
+      program_behaves (I.psem (I.get_interface c) p)  beh.
 End MPC.
 
 (* Software Fault Isolation compiler *)
@@ -364,39 +399,35 @@ Module SFIC <: IT.
   Module T := SFI.
   
   Axiom compile : I.program -> T.program.
-  Axiom compile_complete :
-    forall p1 p2,
-      I.complete p1 -> compile p1 = p2 -> T.complete p2.
-  
-  Axiom compiler_interfaces:
-    forall (p1:I.program),
-      I.get_interface p1 = T.get_interface (compile p1).
+  Axiom compile_spec:
+    forall (p:I.program),
+      I.valid p -> T.valid (compile p) /\
+                   I.get_interface p = T.get_interface (compile p).
 
-  Axiom partialize: interface -> T.program -> option T.program.
-  Axiom partialize_post:
-    forall (p:T.program) psi,
-    exists pp,
-      (T.get_interface p) = (T.get_interface pp)++psi ->
-      partialize psi p = Some pp.
-  Definition opartialize psi (op: option T.program) := propagate (partialize psi) op.
+  Axiom partialize: interface -> T.program -> T.program.
+  Axiom partialize_spec:
+    forall psi (p:T.program),
+      T.valid p ->
+      contained psi (T.get_interface p) ->
+      (T.get_interface p) = (T.get_interface (partialize psi p))++psi.
 
   (* there is no generic decomposition, we need to prove
       special_decomposition *)
   Axiom special_decomposition :
     forall beh (c p:I.program),
       I.fully_defined (I.get_interface c) p ->
-      let ip := map compile (I.link c p) in
-      behaves (T.osem ip) beh
+      let ip := compile (I.link c p) in
+      program_behaves (T.sem ip) beh
       ->
-      behaves (T.opsem (I.get_interface c) (opartialize (I.get_interface c) ip)) beh.
+      program_behaves (T.psem (I.get_interface c) (partialize (I.get_interface c) ip)) beh.
 
   Axiom special_compiler_correctness:
     forall beh (c p:I.program),
       I.fully_defined (I.get_interface c) p ->
       let ip := I.link c p in
-      let tp := opartialize (I.get_interface c) (map compile ip) in
-      behaves (T.opsem (I.get_interface c) tp) beh ->
-      behaves (I.opsem (I.get_interface c) (Some p))  beh.
+      let tp := partialize (I.get_interface c) (compile ip) in
+      program_behaves (T.psem (I.get_interface c) tp) beh ->
+      program_behaves (I.psem (I.get_interface c) p)  beh.
 End SFIC.
 
 
@@ -417,21 +448,27 @@ Module Main (IT : IT).
     forall (c:I.program) (P:S.program) (beh:program_behavior),
       icomplete2 (I.get_interface c) (S.get_interface P) ->
       S.fully_defined (I.get_interface c) P ->
-      behaves (IT.T.osem (map IT.compile (I.link c (SI.compile P)))) beh
+      program_behaves (IT.T.sem (IT.compile (I.link c (SI.compile P)))) beh
       ->
       exists C, 
-        behaves (S.osem (S.link C P)) beh /\ S.complete2 C P.
+        program_behaves (S.sem (S.link C P)) beh /\ S.complete2 C P.
 
   Theorem proof_rc_static : robust_compilation_static_compromise.
   Proof.
     intros c P b Hcomplete SFD H.
     apply (IT.special_decomposition b c (SI.compile P)) in H.
     apply IT.special_compiler_correctness in H.
-    destruct (S.definability b (I.get_interface c) P Hcomplete) as [C [H1 Hinterfaces]].
+    destruct SFD as [HvalP [_ HFD]].
+    destruct (S.definability b (I.get_interface c) P HvalP Hcomplete) as [C [H1 [HvalC Hif]]].
     apply (SI.compiler_correctness b P (I.get_interface c)) in H.
     assumption.
-    rewrite <- Hinterfaces in Hcomplete.
+    assumption.
+    assumption.
+    rewrite <- Hif in Hcomplete.
     exists C.
+    split.
+    auto.
+    unfold S.complete2.
     auto.
     apply SI.FD_preservation.
     assumption.
@@ -447,20 +484,25 @@ Module Main (IT : IT).
       S.complete2 Q P ->
       S.fully_defined (S.get_interface Q) P ->
       let compile := compose IT.compile SI.compile in
-      behaves (IT.T.osem (map compile (S.link Q P))) beh ->
-      exists C, behaves (S.osem (S.link C P)) beh /\ S.complete2 C P.
+      program_behaves (IT.T.sem (compile (S.link Q P))) beh ->
+      exists C, program_behaves (S.sem (S.link C P)) beh /\ S.complete2 C P.
 
   Corollary robust_compilation_corrolary :
     robust_compilation_static_compromise ->
     robust_compilation_static_compromise_corollary.
   Proof.
-    intros RC Q P b Hcompl H1 H2 H3.
+    intros RC Q P b Hcompl SFD H2 H3.
     specialize (RC (SI.compile Q) P b).
-    rewrite <- SI.compiler_interfaces in RC.
-    unfold H2 in H3.
+    assert (SFD2 := SFD).
+    destruct SFD2 as [HvalP [_ HFD]].
+    assert (Hcompl2 := Hcompl).
+    destruct Hcompl2 as [HvalQ [_ Hicompl]].
+    destruct (SI.compile_spec Q).
+    auto.
+    rewrite <- H0 in RC.
     rewrite <- SI.separate_compilation in RC.
-    rewrite <- map_compose in H3.  
-    apply (RC Hcompl H1 H3).
+    apply (RC Hicompl SFD H3).
+    apply Hcompl.
   Qed.
 
 End Main.
